online secrecy: invariant for receive_ping_and_send_ack

dy-extensions/DY.Simplified.fst
@@ -23,11 +23,29 @@ val pk_enc_for:
   traceful (option bytes)
 let pk_enc_for #a alice bob key_sid key_tag plaintext =
   let*? pk_bob = get_public_key alice key_sid (LongTermPkEncKey key_tag) bob in
-  let* nonce = mk_rand PkNonce (principal_label alice) 32 in
+  let* nonce = mk_rand PkNonce (long_term_key_label alice) 32 in
   return ( Some (pk_enc pk_bob nonce (serialize a plaintext)))
 
+// val bytes_invariant_pk_enc_for:
+//   {|protocol_invariants|}->
+//   tr:trace ->
+//   #a:Type -> {|parseable_serializeable bytes a|} ->
+//   alice:principal -> bob:principal ->
+//   alice_pki_sid:state_id ->
+//   key_tag:string ->
+//   msg:a ->
+//   Lemma
+//   (requires
+//       trace_invariant tr
+//   )
+//   (ensures (
+//     let (_, tr_out) = pk_enc_for #a alice bob alice_pki_sid key_tag msg tr in
+//     trace_invariant tr_out
+//   ))
+// let bytes_invariant_pk_enc_for tr #a alice bob alice_pki_sid key_tag msg = ()
+
 val bytes_invariant_pk_enc_for:
-  {|protocol_invariants|}->
+  {|protocol_invariants|} ->
   tr:trace ->
   #a:Type -> {|parseable_serializeable bytes a|} ->
   alice:principal -> bob:principal ->
@@ -35,29 +53,38 @@ val bytes_invariant_pk_enc_for:
   key_tag:string ->
   msg:a ->
   Lemma
-  (requires
+  (requires (
+    let msg_b = serialize #bytes a msg in
       trace_invariant tr
     /\ has_pki_invariant
-    /\ is_knowable_by ( principal_label alice `join` principal_label bob ) tr (serialize a msg)
-    /\ pkenc_pred.pred tr (long_term_key_type_to_usage (LongTermPkEncKey key_tag) bob) (serialize a msg)
-  )
+    /\ bytes_invariant tr msg_b
+    // /\ is_knowable_by ( principal_label alice `join` principal_label bob ) tr (serialize a msg)
+    /\ (get_label tr msg_b) `can_flow tr` (long_term_key_label bob)
+    /\ (get_label tr msg_b) `can_flow tr` (long_term_key_label alice)
+    /\ (pkenc_pred.pred tr (long_term_key_type_to_usage (LongTermPkEncKey key_tag) bob) msg_b
+      \/ (get_label tr msg_b) `can_flow tr` public
+    )
+    ))
   (ensures (
     match pk_enc_for alice bob alice_pki_sid key_tag msg tr with
     | (None, _) -> True
     | (Some cipher, tr_out) -> 
         is_publishable tr_out cipher
   ))
-let bytes_invariant_pk_enc_for #pinvs tr #a alice bob alice_pki_sid key_tag msg =
+let bytes_invariant_pk_enc_for tr #a alice bob alice_pki_sid key_tag msg =
   match pk_enc_for alice bob alice_pki_sid key_tag msg tr with
   | (None, _) -> ()
   | (Some cipher, tr_out) -> (
       let pk_type = LongTermPkEncKey key_tag in
       let (Some pk_bob, _) = get_public_key alice alice_pki_sid pk_type bob tr in
-      let (nonce, tr_nonce) = mk_rand PkNonce (principal_label alice) 32 tr in
+      let (nonce, tr_nonce) = mk_rand PkNonce (long_term_key_label alice) 32 tr in
       let msg = serialize #bytes a msg in
       assert(is_public_key_for tr_out pk_bob pk_type bob);
       let sk_usg = long_term_key_type_to_usage (LongTermPkEncKey key_tag) bob in
-      pkenc_pred.pred_later tr tr_out sk_usg msg
+      introduce pkenc_pred.pred tr sk_usg msg ==> is_publishable tr_out cipher
+      with _ .
+        pkenc_pred.pred_later tr tr_nonce sk_usg msg;
+      ()
 )  
 
 val pk_dec_with_key_lookup:
@@ -71,3 +98,42 @@ let pk_dec_with_key_lookup #a prin keys_sid key_tag cipher =
   let*? plaintext = return (pk_dec sk_a cipher) in 
   // guard_tr ( Some? (parse a plaintext));*?
   return (parse a plaintext)
+
+val bytes_invariant_pk_dec_with_key_lookup:
+  {|protocol_invariants|} ->
+  tr:trace ->
+  #a:Type -> {|parseable_serializeable bytes a|} ->
+  alice:principal -> keys_sid:state_id -> key_tag:string ->
+  cipher:bytes ->
+  Lemma
+  (requires (
+      trace_invariant tr
+    /\ has_private_keys_invariant
+    /\ bytes_invariant tr cipher
+  ))
+  (ensures(
+    match pk_dec_with_key_lookup #a alice keys_sid key_tag cipher tr with
+    | (None, _) -> True
+    | (Some plaintext, _) -> (
+        let plain_b = serialize #bytes a plaintext in
+        is_knowable_by (long_term_key_label alice ) tr plain_b /\
+      ( let sk_usg = (long_term_key_type_to_usage (LongTermPkEncKey key_tag) alice) in
+        ((
+          //PkKey? sk_usg /\
+          pkenc_pred.pred tr sk_usg plain_b )
+          \/ (
+          (get_label tr plain_b `can_flow tr` public)
+        )
+      )
+    )
+  )))
+let bytes_invariant_pk_dec_with_key_lookup tr #a alice keys_sid key_tag cipher = 
+  match pk_dec_with_key_lookup #a alice keys_sid key_tag cipher tr with
+  | (None, _) -> ()
+  | (Some plaintext, _) -> (
+      let (Some sk_alice, _) = get_private_key alice keys_sid (LongTermPkEncKey key_tag) tr in
+      let Some cipher_dec = pk_dec sk_alice cipher in 
+       let sk_usg = (long_term_key_type_to_usage (LongTermPkEncKey key_tag) alice) in
+      bytes_invariant_pk_dec tr sk_alice sk_usg cipher;
+      serialize_parse_inv_lemma a cipher_dec
+  )
