examples/Online_with_secrecy/DY.OnlineS.Invariants.Proofs.fst
@@ -38,3 +38,80 @@ let send_ping_invariant alice bob keys_sid  tr =
       let (sid, tr_sess) = start_new_session alice st tr_msg in
       assert(trace_invariant tr_sess)
   )
+
+val decode_ping_proof:
+  // {|protocol_invariants|} ->
+  tr:trace ->
+  bob:principal -> keys_sid:state_id ->
+  msg:bytes ->
+  Lemma
+  (requires (
+    trace_invariant tr
+    /\ has_private_keys_invariant
+    /\ bytes_invariant tr msg
+  ))
+  (ensures (
+    match decode_ping bob keys_sid msg tr with
+    | (None, _) -> True
+    | (Some png, _) -> (
+        let n_a = png.p_n_a in
+        bytes_invariant tr n_a /\
+        is_knowable_by (nonce_label png.p_alice bob) tr n_a /\
+        ( is_publishable tr n_a
+        \/ (pkenc_pred.pred tr (long_term_key_type_to_usage (LongTermPkEncKey key_tag) bob) (serialize message (Ping png)))
+        )
+    )
+  ))
+let decode_ping_proof tr bob keys_sid msg =
+    match decode_ping bob keys_sid msg tr with
+    | (None, _) -> ()
+    | (Some png, _) -> (
+        bytes_invariant_pk_dec_with_key_lookup tr #message #parseable_serializeable_bytes_message bob keys_sid key_tag msg;
+        let plain = serialize message (Ping png) in
+        parse_wf_lemma message (bytes_invariant tr) plain;
+        FStar.Classical.move_requires (parse_wf_lemma message (is_publishable tr)) plain
+    )
+  
+
+val receive_ping_and_send_ack_invariant:
+  bob:principal -> keys_sid:global_sess_ids -> ts:timestamp ->
+  tr:trace ->
+  Lemma
+  ( requires trace_invariant tr
+  )
+  (ensures (
+    let (_ , tr_out) = receive_ping_and_send_ack bob keys_sid ts tr in
+    trace_invariant tr_out
+  ))
+let receive_ping_and_send_ack_invariant bob bob_keys_sid msg_ts tr =
+  match recv_msg msg_ts tr with
+  | (None, _ ) -> ()
+  | (Some msg, _) -> (
+      match decode_ping bob bob_keys_sid.private_keys msg tr with
+      | (None, _) -> ()
+      | (Some png, _) -> (
+           let n_a = png.p_n_a in
+           let alice = png.p_alice in
+          decode_ping_proof tr bob bob_keys_sid.private_keys msg;
+          assert(is_knowable_by (nonce_label alice bob) tr n_a);
+           let ack = Ack {a_n_a = n_a} in
+           match pk_enc_for bob alice bob_keys_sid.pki key_tag ack tr with
+           | (None, _) -> ()
+           | (Some ack_encrypted, tr_ack) ->(
+                assert(trace_invariant tr_ack);
+                let (ack_ts, tr_msg) = send_msg ack_encrypted tr_ack in
+                serialize_wf_lemma message (bytes_invariant tr) (Ping png);
+                assert(bytes_invariant tr (serialize message (Ping png)));
+                serialize_wf_lemma message (bytes_invariant tr) (ack);
+                assert(bytes_invariant tr (serialize message ack));
+
+                serialize_wf_lemma message (is_knowable_by (nonce_label alice bob) tr) (ack);
+                bytes_invariant_pk_enc_for tr bob alice bob_keys_sid.pki key_tag ack;
+                assert(trace_invariant tr_msg);
+                let st = (SentAck {sa_alice = png.p_alice; sa_n_a = png.p_n_a}) in
+                let (sess_id, tr_sess) = start_new_session bob st tr_msg in
+                //assume(state_predicate_p.pred tr_msg bob sess_id st);
+                assert(trace_invariant tr_sess)
+           )
+      )
+  )
